QR/QR_Iterated_ZK.ec
@@ -1,32 +1,33 @@
 require import AllCore List.
 require import QR_Basics.
-
+import ZK_defs.
 
 require Iterated_Failure.
-clone import Iterated_Failure as IF with type irt <- (qr_c * qr_w),
-                                         type rrt <- bool * bool list,
+clone import Iterated_Failure as IF with type irt <- (qr_prob * qr_wit),
+                                         type rrt <- bool * sbits,
                                          type sbits <- sbits.
 
 
 
 require While_Props.
-clone import While_Props as MW with type irt <- (qr_c * qr_w),
-                                         type rrt <- bool * bool list.
+clone import While_Props as MW with type irt <- (qr_prob * qr_wit),
+                                    type rrt <- bool * sbits.
 
 
 require RewBasics.
 clone import RewBasics as RW with type sbits <- sbits,
                                   type iat   <- iat,
-                                  type iat2  <- (qr_c * qr_w),
-                                  type rrt   <- bool * bool list,
-                                  type irt   <- (qr_c * qr_w),
+                                  type iat2  <- (qr_prob * qr_wit),
+                                  type rrt   <- bool * sbits,
+                                  type irt   <- (qr_prob * qr_wit),
                                   op pair_sbits <- pair_sbits,
                                   op unpair <- unpair.
                                          
 
 module type RewVerifierA = {
-  proc challenge(Ny : qr_c, c : int) : bool 
-  proc summitup(c : int, b : bool, r : int) : bool list 
+  proc challenge(Ny : qr_prob, c : int) : bool 
+  proc summitup(c : int, r : int) : sbits
+  proc verify(c : int, r : int) : bool
   proc getState() : sbits
   proc * setState(b : sbits) : unit 
 }.
@@ -40,7 +41,7 @@ module A(V : RewVerifierA) = {
   proc setState(s : sbits) = {
     V.setState(s);   
   }
-  proc run(i : qr_c * qr_w) : bool * bool list = {
+  proc run(i : qr_prob * qr_wit) : bool * sbits = {
     var r; 
     r <- S.simulate(fst i);
     return r;
@@ -74,16 +75,16 @@ axiom V_challenge_ll : islossless V.challenge.
 lemma qrp_zk2_pr (e ja : int) q &m Na ya wa : 
     IsSqRoot (Na, ya) wa /\ invertible Na ya => 0 <= ja - 2 =>
     ja <= e + 1 =>
-    Pr[ W(A(V)).whp_A(fst, ((Na,ya),wa), 1,e,(false,[])) @ &m :
+    Pr[ W(A(V)).whp_A(fst, ((Na,ya),wa), 1,e,(false,witness)) @ &m :
        W.c = ja /\ (fst res) /\ q (snd res) ]
     = (1%r/2%r)^(ja - 2) * ((1%r/2%r) * Pr[ZK(HP, V).main((Na,ya),wa) @ &m : q res ]).
 move =>  [isr invr] jap1 jap2.
-have <-: Pr[ WW(GetRunSet(A(V))).whp(fst,((Na,ya),wa),1,e,(false,[])) @ &m : WW.c = ja /\ fst res /\ q (snd res) ]  
+have <-: Pr[ WW(GetRunSet(A(V))).whp(fst,((Na,ya),wa),1,e,(false,witness)) @ &m : WW.c = ja /\ fst res /\ q (snd res) ]  
   = Pr[W(A(V)).whp_A(fst, ((Na, ya), wa), 1, e,
-      (false, [])) @ &m : W.c = ja /\ res.`1 /\ q res.`2].
+      (false, witness)) @ &m : W.c = ja /\ res.`1 /\ q res.`2].
 byequiv (_: ={glob A, glob V,arg} ==> WW.c{1} = W.c{2} /\ ={res}).
 proc. sp.  sim. auto. auto.
-apply (whp_cap_fin (GetRunSet(A(V))) A_ll &m fst (fun x => q (snd x)) ((Na,ya),wa) e (false,[]) ja (1%r / 2%r * Pr[ZK(HP, V).main((Na, ya), wa) @ &m : q res]) (fun x => (1%r/2%r)^x))  .
+apply (whp_cap_fin (GetRunSet(A(V))) A_ll &m fst (fun x => q (snd x)) ((Na,ya),wa) e (false,witness) ja (1%r / 2%r * Pr[ZK(HP, V).main((Na, ya), wa) @ &m : q res]) (fun x => (1%r/2%r)^x))  .
 auto. auto. auto. simplify.
 bypr. progress.   
 have <-: 
@@ -104,8 +105,8 @@ byequiv (_: ={arg, glob V, glob Sim1} ==> ={glob Sim1, glob V, res} ). sim. auto
 apply (sim1zk V). apply V_summitup_ll. apply V_challenge_ll. auto. auto. 
 progress. bypr.
 move => &n. elim.  move => ap ge. rewrite ap. simplify.
-have ->: Pr[WW(GetRunSet(A(V))).whp(fst, ((Na,ya),wa), 1, ea, (false,[])) @ &n : ! fst res]
- = Pr[W(A(V)).whp_A(fst, ((Na,ya),wa), 1, ea, (false,[])) @ &m : ! fst res].
+have ->: Pr[WW(GetRunSet(A(V))).whp(fst, ((Na,ya),wa), 1, ea, (false,witness)) @ &n : ! fst res]
+ = Pr[W(A(V)).whp_A(fst, ((Na,ya),wa), 1, ea, (false,witness)) @ &m : ! fst res].
 byequiv (_: ={glob A, glob V,arg} ==> ={res}).
 proc. sp. sim. auto. 
 auto.
