ZK_General.ec
@@ -36,7 +36,7 @@ module type Simulator = {
 
 (* Correctness *)
 module Correct(P : Prover, V : Verifier) = {
-  proc main(Ny:prob, w : wit) = {
+  proc run(Ny:prob, w : wit) = {
     var c,b,r,result;
     c <- P.commit(Ny,w);  
     b <- V.challenge(Ny,c);
@@ -58,3 +58,80 @@ module ZK(P : Prover, V : Verifier) = {
   }
 }.
 
+
+require While_not_b_proc.
+clone import While_not_b_proc as IF with type iat <- (prob * wit),
+                                         type rt <- bool.
+
+(* 
+1/ if one proves soundness
+  forall P &m x, x \notin  L => 
+    Pr[ Correct(P,HV).run(x) @ &m : res ] <= p
+then we can iterate "Correct(P,V).run" (without rewinding)
+to lower probabiliy to success to arbitrary level.
+
+2/ At the same time we also get "completeness"
+since if P succeeds in correctness game with prob. 1
+then iteration preserves it.
+*)
+section.
+declare module P : Prover{M}.
+declare module V : Verifier{M}.
+
+axiom V_verify_ll : islossless V.verify.
+axiom V_challenge_ll : islossless V.challenge.
+axiom P_commit_ll : islossless P.commit.
+axiom P_response_ll : islossless P.response.
+
+
+lemma iterated_correctness_ph (p : real) ia  :  
+ (phoare[ Correct(P,V).run : arg = ia ==> res ] = p) 
+   => forall e, 0 <= e =>
+   phoare[ M(Correct(P,V)).whp : arg = (ia,[!],1,e+1,true) 
+       ==> res ] = (p ^ (e+1)).
+proof. move => H1 e ep .
+have fact1  : phoare[ M(Correct(P,V)).whp_if_end : arg = (ia,[!],1,e,true) ==> res ] = (p ^ (e+1)).
+conseq (asdsad (Correct(P,V)) _  p  ia true [!] _ _ e ep ). 
+proc. 
+call V_verify_ll.
+call P_response_ll.
+call V_challenge_ll.
+call P_commit_ll.
+skip. auto.
+simplify. conseq H1. auto.
+conseq (whp_split_if_end' (Correct(P,V)) _ [!] ia 1 e true (p^(e+1))  (fun x => x) _). 
+proc.
+call V_verify_ll.
+call P_response_ll.
+call V_challenge_ll.
+call P_commit_ll.
+skip. auto.
+apply fact1.
+qed.
+
+lemma iterated_correctness_le_ph (p : real) ia  :  
+ (phoare[ Correct(P,V).run : arg = ia ==> res ] <= p) 
+   => forall e, 0 <= e =>
+   phoare[ M(Correct(P,V)).whp : arg = (ia,[!],1,e+1,true) 
+       ==> res ] <= (p ^ (e+1)).
+proof. move => H1 e ep .
+have fact1  : phoare[ M(Correct(P,V)).whp_if_end : arg = (ia,[!],1,e,true) ==> res ] <= (p ^ (e+1)).
+conseq (asdsad_le (Correct(P,V)) _  p  ia true [!] _ _ e ep ). 
+proc. 
+call V_verify_ll.
+call P_response_ll.
+call V_challenge_ll.
+call P_commit_ll.
+skip. auto.
+simplify. conseq H1. auto.
+conseq (whp_split_if_end_le (Correct(P,V)) _ [!] ia 1 e true (p^(e+1))  (fun x => x) _). 
+proc.
+call V_verify_ll.
+call P_response_ll.
+call V_challenge_ll.
+call P_commit_ll.
+skip. auto.
+apply fact1.
+qed.
+
+end section.
